\section*{Aufgabe 1}
\subsection*{a}
$\alpha$ h\textsubscript{w} $\leq$ h\textsubscript{w} + 6 \newline
Worst Case h\textsubscript{w} = h\textsubscript{w} + 3  \newline
=> $\alpha$ ( h\textsubscript{w} + 3) $\leq$ $\alpha$ h\textsubscript{w} + 6  \newline
$\alpha$ h\textsubscript{w} + $\alpha$ 3 $\leq$ $\alpha$ h\textsubscript{w} + 6  \newline
$\alpha$ 3 $\leq$  6  \newline
$\alpha$ $\leq$  2  \newline
$w\textsubscript{d}  = \begin{cases}
    h\textsubscript{v} - h\textsubscript{w} \leq 3 (a) \\
    h\textsubscript{v} - h\textsubscript{w} \leq 2 (b)
\end{cases}$
$\alpha$ * h\textsubscript{v} $\leq$ $\alpha$ * h\textsubscript{w} + c  \newline
$\alpha$ * (h\textsubscript{w} + d) $\leq$ $\alpha$ * h\textsubscript{w} + c  \newline
$\alpha$ * h\textsubscript{w} + $\alpha$ * d $\leq$ $\alpha$ * h\textsubscript{w} + c  \newline
$\alpha$ * d $\leq$ c  \newline
$\alpha$ $\leq$ $\frac{c}{d}$\newline
=> $\alpha  = \begin{cases}
    2 (a) \\
    3 (b)
\end{cases}$
